Hax/TPhase/CfIntoMonads.lean
@@ -130,7 +130,7 @@ theorem tCfIntoMonads_erase (e : TExpr) :
   | cfBreak _ _ ih => simp [tCfIntoMonads, TExpr.erase, cfIntoMonads, ih]
   | cfContinue _ _ ih => simp [tCfIntoMonads, TExpr.erase, cfIntoMonads, ih]
   | cfBreakContinue _ _ ih => simp [tCfIntoMonads, TExpr.erase, cfIntoMonads, ih]
-  | ann _ _ ih => simp [tCfIntoMonads, TExpr.erase, ih]
+  | ann _ _ ih => simp [tCfIntoMonads, TExpr.erase, cfIntoMonads, ih]
   | namedProj _ _ _ ih =>
     simp [tCfIntoMonads, TExpr.erase, cfIntoMonads, ih]
   | app _ _ args ih =>
